theories/soundness/dyn_getc.v
@@ -16,25 +16,17 @@ From shack.soundness Require Import expr defs.
 Section proofs.
   (* assume a given set of class definitions *)
   Context `{PDC: ProgDefContext}.
+  (* assume some SDT constraints *)
+  Context `{SDTCC: SDTClassConstraints}.
+  (* assume the good properties of SDT constraints *)
+  Context `{SDTCP: SDTClassSpec}.
 
   (* Iris semantic context *)
   Context `{!sem_heapGS Θ}.
 
-  Hypothesis Δsdt_wf: ∀ A vars σ, Forall wf_ty σ → Forall wf_constraint (Δsdt A vars σ).
-  Hypothesis Δsdt_subst_ty: ∀ A vars σ0 σ,
-    subst_constraints σ (Δsdt A vars σ0) = Δsdt A vars (subst_ty σ <$> σ0).
-  Hypothesis Δsdt_bounded: ∀ A vars σ n,
-    Forall (bounded n) σ →
-    Forall (bounded_constraint n) (Δsdt A vars σ).
-  Hypothesis Δsdt_lift: ∀ n A vars σ,
-    lift_constraints n (Δsdt A vars σ) = Δsdt A vars (lift_ty n <$> σ).
-  Hypothesis Δsdt_variance: ∀ Δ kd A vars σ0 σ1,
-    subtype_targs Δ kd vars σ0 σ1 →
-    Δentails kd (Δ ++ Δsdt A vars σ1) (Δsdt A vars σ0).
-
   (* Helping the inference with this notation that hides pdefs *)
-  Local Notation "Δ ⊢ s <: t" := (@subtype _ Δ Plain s t) (at level 70, s at next level, no associativity).
-  Local Notation "Δ ⊢ s <D: t" := (@subtype _ Δ Aware s t) (at level 70, s at next level, no associativity).
+  Local Notation "Δ ⊢ s <: t" := (@subtype _ _ Δ Plain s t) (at level 70, s at next level, no associativity).
+  Local Notation "Δ ⊢ s <D: t" := (@subtype _ _ Δ Aware s t) (at level 70, s at next level, no associativity).
 
   Lemma dyn_get_soundness C Δ kd rigid Γ lhs recv name:
     wf_cdefs pdefs →
@@ -54,7 +46,7 @@ Section proofs.
     |=▷^n heap_models st'.2 ∗ interp_local_tys Σ (<[lhs:=DynamicT]> Γ) st'.1.
   Proof.
     move => wfpdefs ?? hrecv hnotthis Σ st st' n hrigid hc.
-    iIntros "hΣ hΣΔ".
+    iIntros "#hΣ #hΣΔ".
     inv hc.
     iIntros "[Hh #Hle]"; simpl.
     iModIntro. (* keep the later *)
@@ -72,9 +64,9 @@ Section proofs.
     { iDestruct "H" as "%H".
       discriminate H.
     }
-    iDestruct "He" as (dyntag Σdyn dyndef hpure) "[#HΣdyn He]".
+    rewrite interp_sdt_equiv; last by apply wfpdefs.
+    iDestruct "He" as (dyntag Σdyn dyndef hpure) "(#HΣdyn & #hmixed1 & He)".
     destruct hpure as [hdyndef hsupdyn].
-    rewrite interp_tag_equiv; last by apply wfpdefs.
     iDestruct "He" as (?? def def0 ????) "(%H & #hmixed & #hconstr & #hf0 & #hdyn & H◯)".
     destruct H as ([= <-] & hdef & hdef0 & hlen & ? & hinherits & hfields & hidom).
     simplify_eq.
@@ -124,7 +116,7 @@ Section proofs.
         rewrite lookup_app in hc.
         destruct (constraints def0 !! i) as [[??] | ] eqn:h0.
         - rewrite h0 in hc; case: hc => <-.
-          eapply subtype_weaken; [ done | done | | ].
+          eapply subtype_weaken.
           + apply SubConstraint.
             apply elem_of_list_lookup_2 with i.
             by apply h0.
@@ -148,7 +140,6 @@ Section proofs.
         destruct hinherits as (? & ? & ? & hh).
         by apply wf_ty_class_inv in hh.
       }
-      iAssert (interp_env_as_mixed Σdyn) as "hmixed1"; first by admit.
       iAssert (interp_env_as_mixed (interp_list Σt σ)) as "hmixed0".
       { iIntros (k phi hk w) "hphi".
         apply list_lookup_fmap_inv in hk as [ty0 [-> hty0]].
@@ -172,8 +163,7 @@ Section proofs.
         }
         destruct hbc as [].
         rewrite !interp_type_subst //.
-        by iApply ((Δsdt_variance_interp Δsdt_wf Δsdt_subst_ty Δsdt_bounded
-          Δsdt_lift Δsdt_variance _ _ _ _ wf_mono wf_parent hdyndef)
+        by iApply ((Δsdt_variance_interp _ _ _ _ wf_mono wf_parent hdyndef)
           with "hmixed0 hmixed1 hf0 HΣdyn").
       }
       iAssert (□ Σinterp Σt (constraints def0 ++ Δdyn))%I as "hconstr_".
@@ -186,7 +176,7 @@ Section proofs.
       iSpecialize ("h" $! name _ with "[hdyn]"); first done.
       iDestruct "h" as (w) "[%hw hiw]".
       simplify_eq.
-      iDestruct (subtype_is_inclusion _ _ _ _ hwf_ wf_parent wf_mono _ Σt _ _ hsub' v) as "hsub".
+      iDestruct (subtype_is_inclusion _ hwf_ wf_parent wf_mono _ Σt _ _ hsub' v) as "hsub".
       { by apply has_field_wf in hf. }
       by iApply "hsub".
     }
