theories/soundness/dyn_setc.v
@@ -16,10 +16,14 @@ From shack.soundness Require Import expr defs.
 Section proofs.
   (* assume a given set of class definitions *)
   Context `{PDC: ProgDefContext}.
+  (* assume some SDT constraints *)
+  Context `{SDTCC: SDTClassConstraints}.
+  (* assume the good properties of SDT constraints *)
+  Context `{SDTCP: SDTClassSpec}.
 
   (* Helping the inference with this notation that hides pdefs *)
-  Local Notation "Δ ⊢ s <: t" := (@subtype _ Δ Plain s t) (at level 70, s at next level, no associativity).
-  Local Notation "Δ ⊢ s <D: t" := (@subtype _ Δ Aware s t) (at level 70, s at next level, no associativity).
+  Local Notation "Δ ⊢ s <: t" := (@subtype _ _ Δ Plain s t) (at level 70, s at next level, no associativity).
+  Local Notation "Δ ⊢ s <D: t" := (@subtype _ _ Δ Aware s t) (at level 70, s at next level, no associativity).
 
   (* Iris semantic context *)
   Context `{!sem_heapGS Θ}.
@@ -58,20 +62,16 @@ Section proofs.
     { iDestruct "H" as (b) "%H".
       discriminate H.
     }
-    iDestruct "Hl" as "[H | Hl]".
+    iDestruct "Hl" as "[H | He]".
     { iDestruct "H" as "%H".
       discriminate H.
     }
-    iDestruct "Hl" as (dyntag Σdyn dyndef hpure) "Hl".
+    rewrite interp_sdt_equiv; last by apply wfpdefs.
+    iDestruct "He" as (dyntag Σdyn dyndef hpure) "(#HΣdyn & #hmixed1 & He)".
     destruct hpure as [hdyndef hsupdyn].
-    rewrite interp_tag_equiv //; last by apply wfpdefs.
-    iDestruct "Hl" as (?? def def0 ????) "[%H [#hmixed [#hconstr [#hf0 [#hdyn H◯]]]]]".
+    iDestruct "He" as (?? def def0 ????) "(%H & #hmixed & #hconstr & #hf0 & #hdyn & H◯)".
     destruct H as ([= <-] & hdef & hdef0 & hlen & ? & hinherits & hfields & hidom).
     simplify_eq.
-    assert (hwf : wf_ty (ClassT dyntag σ)).
-    { apply inherits_using_wf in hinherits; last by apply wfpdefs.
-      by destruct hinherits as (?&?&?&?).
-    }
     (* This is based on heap_models_update, but specialized for Dynamic *)
     destruct H10 as (vis & fty & orig & hf & hv).
     destruct vis; last by destruct recv.
@@ -123,7 +123,20 @@ Section proofs.
     iRewrite -"hf'".
     iAssert (interp_type DynamicT Σ v) as "#Hve".
     { iApply expr_soundness => //; by apply wfpdefs. }
-    assert (hsub: def0.(constraints) ⊢ DynamicT <D: fty).
+    assert (hl0: length (generics dyndef) = length σ).
+    { apply inherits_using_wf in hinherits; try (by apply wfpdefs).
+      destruct hinherits as (?&?&?&hh).
+      inv hh; by simplify_eq.
+    }
+    pose (Δdyn0 := Δsdt t def0.(generics) (gen_targs (length def0.(generics)))).
+    pose (Δdyn := Δsdt dyntag dyndef.(generics) σ).
+    assert (hnewcond: Δentails Aware (def0.(constraints) ++ Δdyn) Δdyn0).
+    { apply inherits_using_extends_dyn in hinherits => //; try by apply wfpdefs.
+      destruct hinherits as (def0' & ? & hdef0' & ? & hwf); simplify_eq.
+      move => k c hc.
+      by apply hwf with k.
+    }
+    assert (hsub: def0.(constraints) ++ Δdyn0 ⊢ DynamicT <D: fty).
     { destruct wfpdefs.
       assert (h0 := hinherits).
       apply inherits_using_dyn_parent in h0 => //.
@@ -137,11 +150,67 @@ Section proofs.
       apply h1 in hf.
       by apply hf.
     }
-    assert (hwfc: Forall wf_constraint def0.(constraints)) by by apply wf_constraints_wf in hdef0.
+    assert (hsub' : def0.(constraints) ++ Δdyn ⊢ DynamicT <D: fty).
+    { eapply subtype_constraint_trans; first by apply hsub.
+      move => i c hc.
+      rewrite lookup_app in hc.
+      destruct (constraints def0 !! i) as [[??] | ] eqn:h0.
+      - rewrite h0 in hc; case: hc => <-.
+        eapply subtype_weaken.
+        + apply SubConstraint.
+          apply elem_of_list_lookup_2 with i.
+          by apply h0.
+        + by set_solver.
+      - rewrite h0 in hc.
+        by eapply hnewcond.
+    }
     destruct wfpdefs.
-    iDestruct (subtype_is_inclusion _ hwfc wf_parent wf_mono _ Σt _ _ hsub v) as "hsub".
-    { by apply has_field_wf in hf. }
-    iApply "hsub" => //.
+    assert (hwfc: Forall wf_constraint def0.(constraints)) by by apply wf_constraints_wf in hdef0.
+    assert (hwfd: Forall wf_constraint Δdyn).
+    { apply Δsdt_wf.
+      apply inherits_using_wf in hinherits => //.
+      destruct hinherits as (? & ? & ? & hwf); simplify_eq.
+      by apply wf_ty_class_inv in hwf.
+    }
+    assert (hwf_ : Forall wf_constraint (def0.(constraints) ++ Δdyn)).
+    { apply Forall_app; by split.  }
+    assert (hwfσ : Forall wf_ty σ).
+    { apply inherits_using_wf in hinherits => //.
+      destruct hinherits as (? & ? & ? & hh).
+      by apply wf_ty_class_inv in hh.
+    }
+    iAssert (interp_env_as_mixed (interp_list Σt σ)) as "hmixed0".
+    { iIntros (k phi hk w) "hphi".
+      apply list_lookup_fmap_inv in hk as [ty0 [-> hty0]].
+      rewrite -(interp_type_unfold Σt MixedT w).
+      iApply (submixed_is_inclusion_aux Σt ty0 w) => //.
+      rewrite Forall_lookup in hwfσ.
+      by apply hwfσ in hty0.
+    }
+    iAssert (□ Σinterp Σt Δdyn)%I as "#hconstr_dyn".
+    { iClear "Hle hdyn H◯ Hv hifs hmodfs hf' Hve".
+      iModIntro; iIntros (i c0 hc w) "#h".
+      rewrite /Δdyn -(subst_ty_gen_targs (length dyndef.(generics)) σ) // in hc.
+      rewrite -Δsdt_subst_ty in hc.
+      apply list_lookup_fmap_inv in hc as [c [-> hc]] => /=.
+      assert (hbc : bounded_constraint (length σ) c).
+
+      { rewrite -hl0.
+        move : (bounded_gen_targs (length dyndef.(generics))) => hh.
+        apply Δsdt_bounded with (A := dyntag) (vars := dyndef.(generics)) in hh.
+        rewrite Forall_lookup in hh.
+        by apply hh in hc.
+      }
+      destruct hbc as [].
+      rewrite !interp_type_subst //.
+      by iApply ((Δsdt_variance_interp _ _ _ _ wf_mono wf_parent hdyndef)
+      with "hmixed0 hmixed1 hf0 HΣdyn").
+    }
+    iAssert (□ Σinterp Σt (constraints def0 ++ Δdyn))%I as "hconstr_".
+    { iModIntro.
+      by iApply Σinterp_app.
+    }
+    iApply (subtype_is_inclusion _ hwf_ wf_parent wf_mono _ Σt _ _ hsub' v) => //.
     by rewrite !interp_dynamic_unfold.
   Qed.
 End proofs.
