theories/soundness/sub.v
@@ -16,16 +16,13 @@ From shack.soundness Require Import defs.
 Section proofs.
   (* assume a given set of class definitions *)
   Context `{PDC: ProgDefContext}.
+  (* assume some SDT constraints *)
+  Context `{SDTCC: SDTClassConstraints}.
+  (* assume the good properties of SDT constraints *)
+  Context `{SDTCP: SDTClassSpec}.
 
   (* Iris semantic context *)
   Context `{!sem_heapGS Θ}.
-
-  Hypothesis Δsdt_wf: ∀ A vars σ, Forall wf_ty σ → Forall wf_constraint (Δsdt A vars σ).
-  Hypothesis Δsdt_subst_ty: ∀ A vars σ0 σ,
-    subst_constraints σ (Δsdt A vars σ0) = Δsdt A vars (subst_ty σ <$> σ0).
-  Hypothesis Δsdt_bounded: ∀ A vars σ n,
-    Forall (bounded n) σ →
-    Forall (bounded_constraint n) (Δsdt A vars σ).
 
   Lemma sub_soundness C Δ kd Γ rigid Γ0 Γ1 c:
     wf_cdefs pdefs →
